src/Trace.v
@@ -1,0 +1,23 @@
+Set Implicit Arguments.
+
+Require Import Tid.
+Require Import Mid.
+
+Section Defs.
+  Inductive datum :=
+  | d_task : tid -> datum
+  | d_mem : mid -> datum
+  | d_any : datum.
+
+  Inductive op :=
+  | CONTINUE: op
+  | ALLOC: mid -> datum -> op
+  | READ: mid -> datum -> op
+  | WRITE: mid -> datum -> op
+  | FUTURE: tid -> list datum -> op
+  | FORCE: tid -> datum -> op.
+
+  Definition event := (tid * op) % type.
+
+
+End Defs.
